theories/simd.v
@@ -6,8 +6,18 @@ Set Implicit Arguments.
 Unset Strict Implicit.
 Unset Printing Implicit Defensive.
 
-Module Type SIMD.
+Module Type SIMD_Type.
 
-Parameter v128: Type.
+  Parameter v128: Type.
 
+  Parameter v128_default: v128.
+
+End SIMD_Type.
+
+Module SIMD <: SIMD_Type.
+
+  Definition v128 := bytes.
+
+  Definition v128_default : v128 := nil.
+  
 End SIMD.
